theories/L6_PCPS/Heap/toplevel.v
@@ -1,0 +1,189 @@
+From L6 Require Import cps cps_util set_util identifiers ctx Ensembles_util
+     List_util functions tactics.
+
+From L6.Heap Require Import heap heap_defs heap_equiv space_sem
+     cc_log_rel closure_conversion closure_conversion_util bounds
+     invariants GC closure_conversion_correct.
+
+From Coq Require Import ZArith.Znumtheory Relations.Relations Arith.Wf_nat
+                        Lists.List MSets.MSets MSets.MSetRBT Numbers.BinNums
+                        NArith.BinNat PArith.BinPos Sets.Ensembles Omega Permutation.
+
+Import ListNotations.
+
+Open Scope ctx_scope.
+Open Scope fun_scope.
+Close Scope Z_scope.
+
+Module Top (H : Heap).
+
+  Module CC := ClosureConversionCorrect H.
+  
+  Import H CC.Inv.Size.Util.C.LR.Sem.GC.Equiv
+         CC.Inv.Size.Util.C.LR.Sem.GC.Equiv.Defs
+         CC.Inv.Size.Util.C.LR.Sem.GC CC.Inv.Size.Util.C.LR.Sem
+         CC.Inv.Size.Util.C.LR CC.Inv.Size.Util.C CC.Inv.Size.Util
+         CC.Inv.Size CC.Inv CC.
+
+  Definition ct := CC.Inv.Size.Util.clo_tag. 
+
+  (** The expression relation is monotonic in the local invariant *)
+  Lemma cc_approx_exp_rel_mon k j LIP1 LIP2 GIP1 (LP1 : Inv) (GP1 : GInv)
+        (p1 p2 : exp * env * heap block) :
+    p1 ⪯ ^ ( k ; j ; LIP1 ; GIP1 ; LP1 ; GP1 ) p2 ->
+    inclusion _ LIP2 LIP1 ->
+    p1 ⪯ ^ ( k ; j ; LIP2 ; GIP1 ; LP1 ; GP1 ) p2.
+  Proof.
+    destruct p1 as [[e1 H1] rho1].
+    destruct p2 as [[e2 H2] rho2]. 
+    intros Hcc Hin b1 b2 H1' H2' rho1' rho2' v1 c1 m1 HH1 Hr1 HH2 Hr2 Hip Hleq Hstep Hstuck.
+    edestruct Hcc as [v2 [c2 [m2 [b' [Hstep' [HInv Hval]]]]]]; eauto.
+  Qed.
+
+  Definition instal_env Γ :=
+    let (lenv, H1) := alloc (Constr ct []) emp in
+    (M.set Γ (Loc lenv) (M.empty _), H1).
+
+  Lemma key_set_empty A :
+    key_set (M.empty A) <--> Empty_set _.
+  Proof. 
+    split; eauto with Ensembles_DB.
+    intros x k. unfold In, key_set in *.
+    rewrite M.gempty in k. contradiction.
+  Qed.
+
+  Lemma closure_conversion_correct_lr_closed (k : nat) (e1 e2 : exp) (C : exp_ctx) (Γ : var) K rho2 H2 :
+    (rho2, H2) = instal_env Γ ->
+    ~ Γ \in bound_var e1 ->
+    unique_bindings e1 ->
+    
+    Closure_conversion ct (Empty_set _) (Empty_set _) id ct Γ [] e1 e2 C ->
+    
+    (forall j, (e1, M.empty _, emp) ⪯ ^ (k ; j ;
+                              Pre (Empty_set _) K; Pre;
+                              Post 0 K; Post 0)
+          (C |[ e2 ]|, rho2, H2)).
+  Proof with (now eauto with Ensembles_DB).
+    unfold instal_env.
+    destruct (alloc (Constr ct []) emp) as [lenv Η2] eqn:Ha. 
+    intros Ha' Hnin Hun Hcc. inv Ha'. 
+    intros j.
+    eapply Closure_conversion_correct in Hcc.
+    eapply cc_approx_exp_rel_mon.
+    - eassumption. 
+    - eapply Pre_subset_compat.
+      rewrite Intersection_Empty_set_abs_l...
+    - tci.
+    - intros j1. eapply cc_approx_env_Empty_set.
+    - intros j2. split.
+      + rewrite env_locs_set_In, <- env_locs_Empty; [| reflexivity ].
+        rewrite !Union_Empty_set_neut_r.
+        rewrite reach_unfold.
+        simpl. rewrite post_Singleton; [| eapply gas; eassumption ].  
+        simpl. rewrite reach'_Empty_set.
+        rewrite !Union_Empty_set_neut_r.
+        intros x b Hi Hget; inv Hi. eapply gas in Ha.
+        subst_exp...
+      + split.
+        * unfold FV.
+          rewrite key_set_empty.
+          rewrite FromList_nil, !Setminus_Empty_set_neut_r. 
+          rewrite !Union_Empty_set_neut_r at 1.
+          rewrite Setminus_Empty_set_neut_r, !Union_Empty_set_neut_r.
+          reflexivity.
+        * do 2 eexists. split; [| split ].
+          rewrite M.gss. reflexivity. 
+          eapply gas. eassumption.
+          now constructor. 
+    - intros j1 x _ Hin. inv Hin.
+    - unfold FV.
+      rewrite FromList_nil, !Setminus_Empty_set_neut_r, !image_Empty_set, !Union_Empty_set_neut_r at 1.
+      rewrite Setminus_Empty_set_neut_r, !Union_Empty_set_neut_r.
+      eapply Disjoint_Singleton_l. eassumption.
+    - unfold FV.
+      rewrite FromList_nil, !Setminus_Empty_set_neut_r. 
+      rewrite !Union_Empty_set_neut_r at 1.
+      rewrite Setminus_Empty_set_neut_r, !Union_Empty_set_neut_r.
+      intros x Hin. inv Hin.
+    - eassumption.
+    - unfold FV.
+      rewrite FromList_nil, !Setminus_Empty_set_neut_r. 
+      rewrite !Union_Empty_set_neut_r at 1.
+      rewrite Setminus_Empty_set_neut_r, !Union_Empty_set_neut_r.
+      now eauto with Ensembles_DB.
+
+      Grab Existential Variables.
+      tci. exact id.
+  Qed.
+
+  (** ** Top-level theorem *) 
+  
+  Lemma closure_conversion_correct_top
+        (k : nat) (j : nat) (e1 e2 : exp) (C : exp_ctx) (Γ : var) (* dummy varaiable for environment *)
+        H2 rho2 r1 c1 m1 :
+    
+    (rho2, H2) = instal_env Γ ->
+    ~ Γ \in bound_var e1 ->
+    (* The source program has unique binders *)
+    unique_bindings e1 ->
+
+    (* C[e2] is the closure converted program *)
+    Closure_conversion ct (Empty_set _) (Empty_set _) id ct Γ [] e1 e2 C ->
+
+    (* the source evaluates *)
+    big_step_GC emp (M.empty _) e1 r1 c1 m1 ->
+    (* and it is not a stuck program *)
+    not_stuck emp (M.empty _) e1 ->
+    
+    exists (r2 : ans) (c2 m2 : nat) (b : Inj),
+      (* the target evaluates *)
+      big_step_GC_cc H2 rho2 (C |[ e2 ]|) r2 c2 m2 /\
+      (* time bounds *)
+      c1 <= c2 <= c1 * (1 + cost_time_exp e1) + (cost_time_exp e1) /\
+      (* space bounds *)
+      m2 <= m1 * (1 + (cost_mem_exp e1)) + 2 * (1 + (cost_mem_exp e1)) /\
+      (* the results are related *)
+      r1 ≺ ^ (k ; j ; Pre ; Post 0 ; b ) r2.  
+  Proof with (now eauto with Ensembles_DB).
+    unfold instal_env.
+    destruct (alloc (Constr ct []) emp) as [lenv H2'] eqn:Ha. 
+    intros Ha' Hnin Hun Hcc Hbs Hns. inv Ha'. 
+    assert (Heq : (e1, M.empty _, emp) ⪯ ^ (k + c1 ; j ;
+                                            Pre (Empty_set _) 1; Pre;
+                                            Post 0 1; Post 0)
+                  (C |[ e2 ]|, (M.set Γ (Loc lenv) (M.empty value)), H2')).
+    { eapply closure_conversion_correct_lr_closed; try eassumption.
+      unfold instal_env. rewrite Ha. reflexivity. }
+
+    edestruct Heq as (r2 & c2 & m2 & b & Hbs2 & Hin & Hres).
+    - reflexivity.
+    - clear; now firstorder.
+    - reflexivity.
+    - clear; now firstorder.
+    - unfold Pre. unfold size_heap, size_cc_heap.
+      rewrite !HL.size_with_measure_emp. rewrite !plus_O_n at 1.
+      rewrite PS_cardingal_empty.
+      simpl. rewrite <- plus_n_O.
+      erewrite HL.size_with_measure_alloc with (s := 0); try eassumption. 
+      simpl. omega.
+      eapply HL.size_with_measure_emp. 
+      rewrite <- mset_eq. reflexivity. 
+    - eapply le_plus_r.
+    - eassumption.
+    - eassumption.
+    - unfold Post in Hin. destruct Hin as [[Ht1 Ht2] Hm]. do 4 eexists. split. eassumption.
+      split; [| split ].
+      + split. omega. unfold cost_time_heap, cost_heap in *.
+        rewrite HL.max_with_measure_emp in *. rewrite <- !plus_n_O, !Max.max_0_r in *.
+        omega.
+      + unfold cost_mem_heap, cost_heap in *.
+        rewrite HL.max_with_measure_emp in *. rewrite <- !plus_n_O, !Max.max_0_r in *.
+        eapply le_trans. eassumption. eapply plus_le_compat_l.
+        eapply mult_le_compat_l. eapply Max.max_lub. omega. omega. 
+      + rewrite cc_approx_val_eq in Hres.
+        eapply cc_approx_val_monotonic. eassumption. omega.
+  Qed.
+
+  Print Assumptions closure_conversion_correct_top.
+
+End Top. 
